src/computability/partrec.lean
@@ -569,6 +569,13 @@ theorem option_get_or_else {f : α → option β} {g : α → β}
 (computable.option_cases hf hg (show computable₂ (λ a b, b), from computable.snd)).of_eq $
 λ a, by cases f a; refl
 
+theorem subtype_mk {f : α → β} {p : β → Prop} [decidable_pred p] {h : ∀ a, p (f a)}
+    (hp : primrec_pred p) (hf : computable f) :
+  @computable _ _ _ (primcodable.subtype hp) (λ a, (⟨f a, h a⟩ : subtype p)) :=
+option_some_iff.1 $ _
+
+#exit
+
 theorem sum_cases
   {f : α → β ⊕ γ} {g : α → β → σ} {h : α → γ → σ}
   (hf : computable f) (hg : computable₂ g) (hh : computable₂ h) :
